# Soundness


We will now show that the extension is sound. To do so we first will show the soundness of the new semantic with respect to the inference rules. 

```{theorem}
\label{thm:soundness_int_exp_type}
\begin{letIn}
$\mathit{iet} \in\mf{<int-exp-type>}$ and $\mathit{exp}\in\mathit{IntExp}$. Assume $\mathit{iet}:\mathit{exp}$ can be derived.
\end{letIn}
Then \(\semantic{$\mathit{iet}$} = \mathit{exp}\).
```
```{proof}
Let $\mathit{iet} \in\mf{<int-exp-type>}$ and $\mathit{exp}\in\mathit{IntExp}$. Assume $\mathit{iet}:\mathit{exp}$ can be derived.
\begin{itemize}
    \item \textbf{Case} $\mathit{iet} = i$ for $i\in\mathit{Int}$: Then $\semantic{$\mathit{iet}$} = i$ and therefore the conclusion holds.
    \item \textbf{Case} $\mathit{iet} = \mathit{iet}_1 \ \mf{+} \ \mathit{iet}_2$ for $\mathit{iet}_1,\mathit{iet}_2 \in\mf{<int-exp-type>}$: From the premise of the inference rule, we assume that $\mathit{iet}_1:\mathit{exp}_1$ and $\mathit{iet}_2:\mathit{exp}_2$ hold. By induction hypothesis $\semantic{$\mathit{iet}_1$} = \mathit{exp}_1$ and $\semantic{$\mathit{iet}_2$} = \mathit{exp}_2$. Thus $\semantic{$\mathit{iet}$} = \mathit{exp}_1 + \mathit{exp}_2$ and therefore the conclusion holds.
    \item \textbf{Case} $\mathit{iet} = \mathit{iet}_1 \ \mf{*} \ i$ for $\mathit{iet}_1\in\mf{<int-exp-type>}$ and $i\in\mathit{Int}$: From the premise of the inference rule, we assume that $\mathit{iet}_1:\mathit{exp}_1$ holds. By induction hypothesis $\semantic{$\mathit{iet}_1$} = \mathit{exp}_1$. Thus $\semantic{$\mathit{iet}$} = \mathit{exp}_1 \cdot i$ and therefore the conclusion holds.
    \item \textbf{Case} $\mathit{iet} = a$ for $a\in\mathcal{V}$: Then $\semantic{$a$} = a$ and therefore the conclusion holds.
\end{itemize}
```

```{theorem}
\label{thm:soundness_qualifier_type}
\begin{letIn}
$\mathit{qt} \in\mf{<qualifier-type>}$ and $q\in\mathcal{Q}$. Assume $\mathit{qt}:q$ can be derived.
\end{letIn}
Then \(\semantic{$\mathit{qt}$} = q\).
```
```{proof}
Let $\mathit{qt} \in\mf{<qualifier-type>}$ and $q\in\mathcal{Q}$. Assume $\mathit{qt}:q$ can be derived.
\begin{itemize}
    \item \textbf{Case} $\mathit{qt} = \mf{True}$: Then $\semantic{$\mathit{qt}$} = \mathit{True}$ and therefore the conclusion holds.
    \item \textbf{Case} $\mathit{qt} = \mf{False}$: Then $\semantic{$\mathit{qt}$} = \mathit{False}$ and therefore the conclusion holds.
    \item \textbf{Case} $\mathit{qt} = \mf{(<)} \ \mathit{iet} \ \mf{v}$: From the premise of the inference rule, we assume that $\mathit{iet}:\mathit{exp}$. By Theorem \ref{thm:soundness_int_exp_type} $\semantic{$\mathit{iet}$} = \mathit{exp}$ for $\mathit{exp}\in\mathit{IntExp}$. Then $\semantic{$\mathit{qt}$} = \mathit{exp} < \nu$ and therefore the conclusion holds.
    \item \textbf{Case} $\mathit{qt} = \mf{(<)} \ \mf{v} \ \mathit{iet} $: From the premise of the inference rule, we assume that $\mathit{iet}:\mathit{exp}$. By Theorem \ref{thm:soundness_int_exp_type} $\semantic{$\mathit{iet}$} = \mathit{exp}$ for $\mathit{exp}\in\mathit{IntExp}$. Then $\semantic{$\mathit{qt}$} = \nu < \mathit{exp}$ and therefore the conclusion holds.
    \item \textbf{Case} $\mathit{qt} = \mf{(=)} \ \mf{v} \ \mathit{iet} $: From the premise of the inference rule, we assume that $\mathit{iet}:\mathit{exp}$. By Theorem \ref{thm:soundness_int_exp_type} $\semantic{$\mathit{iet}$} = \mathit{exp}$ for $\mathit{exp}\in\mathit{IntExp}$. Then $\semantic{$\mathit{qt}$} = (\nu = \mathit{exp})$ and therefore the conclusion holds.
    \item \textbf{Case} $\mathit{qt} = \mf{(\&\&)}\ \mathit{qt}_1 \ \mathit{qt}_2$ for $\mathit{qt}_1,\mathit{qt}_2 \in \mf{<qualifier-type>}$: From the premise of the inference rule, we assume that $\mathit{qt}_1:q_1$ and $\mathit{qt}_2:q_2$ hold for $q_1,q_2\in\mathcal{Q}$. By induction hypothesis $\semantic{$\mathit{qt}_1$} = q_1$ and $\semantic{$\mathit{qt}_2$} = q_2$. Thus $\semantic{$\mathit{qt}$} = q_1 \land q_2$ and therefore the conclusion holds.
    \item \textbf{Case} $\mathit{qt} = \mf{(||)}\ \mathit{qt}_1 \ \mathit{qt}_2$ for $\mathit{qt}_1,\mathit{qt}_2 \in \mf{<qualifier-type>}$: From the premise of the inference rule, we assume that $\mathit{qt}_1:q_1$ and $\mathit{qt}_2:q_2$ hold for $q_1,q_2\in\mathcal{Q}$. By induction hypothesis $\semantic{$\mathit{qt}_1$} = q_1$ and $\semantic{$\mathit{qt}_2$} = q_2$. Thus $\semantic{$\mathit{qt}$} = q_1 \lor q_2$ and therefore the conclusion holds.
    \item \textbf{Case} $\mathit{qt} = \mf{not} \ \mathit{qt}_1$ for $\mathit{qt}_1\in\mf{<qualifier-type>}$: From the premise of the inference rule, we assume that $\mathit{qt}_1:q_1$ holds for $q_1\in\mathcal{Q}$. By induction hypothesis $\semantic{$\mathit{qt}_1$} = q_1$. Thus $\semantic{$\mathit{qt}$} = \neg \ q_1$ and therefore the conclusion holds.
\end{itemize}
```

```{theorem}
\label{thm:soundness_liquid_type}
\begin{letIn}
$\Theta:\mathcal{V}\nrightarrow\mathcal{Q}$. Let $\mathit{lt} \in\mf{<liquid-type>}$ and $\hat{T}\in\mathcal{T}$. Assume $\mathit{lt}:_\Theta\hat{T}$ can be derived.
\end{letIn}
Then \(\semantic{$\mathit{lt}$} = \hat{T}\).
```
```{proof}
Let $\Theta:\mathcal{V}\nrightarrow\mathcal{Q}$. Let $\mathit{lt} \in\mf{<liquid-type>}$ and $\hat{T}\in\mathcal{T}$. Assume $\mathit{lt}:_\Theta\hat{T}$ can be derived.
\begin{itemize}
    \item \textbf{Case} $\mathit{lt} = \mf{"\{v:Int|"}\ \mathit{qt} \ \mf{"\}"}$ for $\mathit{qt}\in\mf{<qualifier-type>}$: From the premise of the inference rule, we assume that $\mathit{qt}:q$ for $q\in\mathcal{Q}$ holds. By Theorem \ref{thm:soundness_qualifier_type} $\semantic{$\mathit{qt}$}=q$. Then $\semantic{$\mathit{lt}$} = \{\nu:\mathit{Int}| \ q\}$ and therefore the conclusion holds.
    \item \textbf{Case} $\mathit{lt} = a \ \mf{":"} \ \mf{"\{v:Int|"}\ \mathit{qt} \ \mf{"\}"} \ \mf{"->"} \ \mathit{lt}_2$ for $a\in\mathcal{V}, \mathit{qt}\in\mf{<qualifier-type>}$ and $\mathit{lt}\in\mf{<liquid-type>}$: From the premise of the inference rule, we assume that $\mf{"\{v:Int|"}\ \mathit{qt} \ \mf{"\}"}:_\Theta\{\nu:\mathit{Int}|r_1\}$ and $\mathit{lt}_2:_{\Theta\cup\{(a,r_1)\}}\hat{T}_2$ for liquid type $\hat{T}_2$ and $r_1\in\mathcal{Q}$. By induction hypothesis $\semantic{$\mathit{lt}_2$} = \hat{T}_2$. Then $\semantic{$\mathit{lt}$} = a:\{\nu:\mathit{Int}|r_1\}\to\hat{T}_2$ and therefore the conclusion holds.
\end{itemize}
```

We can now again prove the soundness of the semantic of type annotations.

```{theorem}
\begin{letIn}
$\Gamma$ be a type context, $t \in\mf{<type>}$ and $T\in\mathcal{T}$. Assume $\Gamma\vdash t:T$ can be derived.
\end{letIn}
Then \(\semantic{$t$}_\Gamma = T\).
```
```{proof}
Let $\Gamma$ be a type context, $t \in\mf{<type>}$ and $T\in\mathcal{T}$. Assume $\Gamma\vdash t:T$ can be derived.
\begin{itemize}
    \item \textbf{Case} $t = \mathit{lt}$ for $\mathit{lt}\in\mf{<liquid-type>}$: From the premise of the inference rule, we assume that $\mathit{lt}:_\Theta\hat{T}$ for liquid type $\hat{T}$ holds. By Theorem \ref{thm:soundness_liquid_type} $\semantic{$\mathit{lt}$} = \hat{T}$. Then $\semantic{$\mathit{t}$} = \hat{T}$ and therefore the conclusion holds.
\end{itemize}

All other cases have been proven in Theorem \ref{thm:soundness_type}.
```

What is left is to prove the soundness of the semantic of expressions. This is by the definition of refinement types trivially true, as the set values of a refinement type is always a subtype of the set of values of the base type.

```{theorem}
\begin{letIn}
$\Gamma,\Delta$ be type contexts, $\Delta'$ be a variable context similar to $\Delta$ with respect to $\Gamma$. Let $\Lambda\subset\mathcal{Q}$ and $\Theta:\mathcal{V}\nrightarrow\mathcal{Q}$. Let $e\in\mf{<exp>}$ and $T\in\mathcal{T}$. Assume $\Gamma,\Delta,\Theta,\Lambda\vdash e:T$ can be derived. 
\end{letIn}
Then \(\semantic{$e$}_{\Gamma,\Delta'}\in\text{value}_\Gamma(\overline{\Gamma}(T))\).
```
```{proof}
Let $\Gamma,\Delta$ be type contexts, $\Delta'$ be a variable context similar to $\Delta$ with respect to $\Gamma$. Let $\Lambda\subset\mathcal{Q}$ and $\Theta:\mathcal{V}\nrightarrow\mathcal{Q}$. Let $e\in\mf{<exp>}$ and $T\in\mathcal{T}$. Assume $\Gamma,\Delta,\Theta,\Lambda\vdash e:T$ can be derived.
\begin{itemize}
    \item \textbf{Case} $e = \mf{"(+)"}$: Then $T =a:\mathit{Int}\to b:\mathit{Int}\to\{\nu:\mathit{Int} \ | \ \nu = a + b\}$ and $\semantic{"(+)"}_{\Gamma,\Delta'} = \lambda n.\lambda m. n + m$ where $n,m\in\mathbb{Z}$ and thus the conclusion holds.
    \item \textbf{Case} $e = \mf{"(-)"}$: Then $T =a:\mathit{Int}\to b:\mathit{Int}\to\{\nu:\mathit{Int} \ | \ \nu = a + (-b)\}$ and \(\semantic{"(-)"}_{\Gamma,\Delta'} = \lambda n.\lambda m. n - m\) where $n,m\in\mathbb{Z}$ and thus by $n - m = n + (-m)$ the conclusion holds.
    \item \textbf{Case} $e = \mf{"(*)"}$: Then $T = a:\mathit{Int}\to b:\mathit{Int}\to\{\nu:\mathit{Int} \ | \ \nu = a * b\}$ and \(\semantic{"(*)"}_{\Gamma,\Delta'} = \lambda n.\lambda m. n * m\) where $n,m\in\mathbb{Z}$
and thus the conclusion holds.
    \item \textbf{Case} $e = \mf{"(//)"}$: Then $T = \mathit{Int}\to\{\nu:\mathit{Int} \ | \ \neg (\nu = 0)\}\to\mathit{Int}$ and \[\semantic{"(//)"}_{\Gamma,\Delta'} = s:\Leftrightarrow 
s = \lambda n.\lambda m.\begin{cases} \Big\lfloor \frac{n}{m} \Big\rfloor& \text{if } m \neq 0\\
        0& \text{else}\end{cases}\] where $n,m\in\mathbb{Z}$. Wee see that the "else"-case is dead and the $m \neq 0$-case is well formed. Thus the conclusion holds
    \item \textbf{Case} $e = \mf{"if"} \ e_1  \ \mf{"then"} \ e_2 \ \mf{"else"} \ e_3$ for $e_1,e_2,e_3\in\mf{<exp>}$: By the premise of the inference rule we assume $\Gamma,\Delta,\Theta,\vdash e_1:\textit{Bool}$, $\Gamma,\Delta,\Theta,\Lambda\cup\{e_1'\}\vdash e_2: \hat{T}$ and $\Gamma,\Delta,\Theta,\Lambda\cup\{\neg e_1'\}\vdash e_3: \hat{T}$ as well as  $e_1:e_1'$ can be derived for $e_1'\in\mathcal{Q}$. By induction hypothesis $\semantic{$e_1$}_{\Gamma,\Delta'} \in \text{value}(\textit{Bool})$, $\semantic{$e_2$}_{\Gamma,\Delta'} \in \text{value}(T)$ and $\semantic{$e_3$}_{\Gamma,\Delta'} \in \text{value}(T)$.  Thus, by the definition of the semantics the conclusion holds analogously to the cases above.
    \item \textbf{Case} $e = e_1 \ e_2$ for $e_1,e_2\in\mf{<exp>}$: By the premise of the inference rule we assume $\Gamma,\Delta,\Theta,\Lambda\vdash e_1: (a:\hat{T}_1\to \hat{T}_2)$ and  $\Gamma,\Delta,\Theta,\Lambda\vdash e_2: \hat{T}_1$ as well as $[\hat{T}_2]_{a\leftarrow e_2'} =T$ and $e_2:e_2'$  can be derived for $e_2'\in\mathcal{Q}$ and $a\in\mathcal{V}$. Therefore, by the induction hypothesis we know, \(\semantic{$e_1$}_{\Gamma,\Delta'}\in\text{value}_\Gamma(\overline{\Gamma}(\hat{T}_1\to \hat{T}_2))\) and \(\semantic{$e_1$}_{\Gamma,\Delta'}\in\text{value}_\Gamma(\overline{\Gamma}(\hat{T}_1))\). Thus $\semantic{$e$}\in\text{value}([\hat{T}_2]_{a\leftarrow e_2'})$ and thus the semantics the conclusion holds analogously to the cases above.
    \item \textbf{Case} $e = \mf{"\textbackslash"} \ a \ \mf{"->"} \ e$ for $a\in\mathcal{V},e\in\mf{<exp>}$: Then $T = b:\{\nu:\mathit{Int}|r_1\} \to \hat{T}_2$ for liquid types $\hat{T}_1,\hat{T}_2$ and $b\in\mathcal{V}$. By the premise of the inference rule we assume  $\Gamma,\Delta\cup\{(a,\{\nu:\mathit{Int}|r_1\})\},\Theta\cup\{(a,r_1)\},\Lambda\vdash e: \hat{T}_2$ can be derived. We now need to show that \(\semantic{$e$}_{\Gamma,\Delta'}\in\text{value}_\Gamma(\{\nu:\mathit{Int}|r_1\}\to \hat{T}_2)\). We know \(\semantic{$e$}_{\Gamma,\Delta'}=\lambda b. \semantic{$e$}_{\Gamma,\Delta\cup\{(a,b)\}}\) for $b\in\mathcal{V}$. We will therefore by the definition of the abstraction in the lambda expression let $b\in\text{value}_\Gamma(\overline{\Gamma}(\{\nu:\mathit{Int}|r_1\}))$ and show \(\semantic{$e$}_{\Gamma,\Delta'\cup\{(a,b)\}}\in\text{value}_\Gamma(\hat{T}_2)\). By Theorem \ref{thm:similar_variable_context} $\Delta'\cup\{(a,b)\}$ is similar to $\Delta\cup\{(a,\overline{\Gamma}(\hat{T}_1))\}$ and therefore by induction hypothesis we conclude \(\semantic{$e$}_{\Gamma,\Delta'\cup\{(a,b)\}}\in\text{value}_\Gamma(\hat{T}_2)\). Thus the conclusion holds.
    \item \textbf{Case} $e = a$ for $a\in\mathcal{V}$: By the premise of the inference rule we assume $(c,T)\in\Delta$. The semantic requires that there exists an $e\in\text{value}_\Gamma(\overline{\Gamma}(T))$ such that $(c,e)\in\Delta'$.
$\Delta'$ is similar to $\Delta$ and therefore this is a valid assumption. Thus, the semantic is sound and by its definition the conclusion holds analogously to the cases above.
\end{itemize}

All other cases have been proven in Theorem \ref{thm:soundness_type}.
```