\setcounter{section}{3}
\setcounter{subsection}{3}

## Denotational Semantic

We will now expore the semantics of the formal language. To do so, we first define a new context.

```{definition, name="Variable Context"}
\begin{letIn}
$\Gamma$ be a type context.
\end{letIn}
$\Delta : \mathcal{V} \nrightarrow \bigcup_{T\in\mathcal{T}}\text{value}_\Gamma(T)$ is called a _variable context_.
```

The semantics of the type signature was already defined in the last section, as the semantic of a type signature is its type. We therefore define the same concept but now in a denotational style.

```{definition, name="Type Signature Semantic"}
\begin{letIn}
$T,T'\in\mathcal{T}$, $c,a_0,a\in\mathcal{V}$. Let $t_0,t_1,t_2\in\mf{<type>}$, $ltf\in\mf{<list-type-fields>}$ and $lt\in\mf{<list-type>}$. Let $\Gamma$ be a type context.
\end{letIn}

Let $s\in(\mathcal{V}\times\mathcal{T})^*$ for the following function.

$$
\begin{aligned}
\semantic{.}_\Gamma:&\mf{<list-type-fields>}\to(\mathcal{V}\times\mathcal{T})^*\\
\semantic{""}_\Gamma = s :\Leftrightarrow
    & s = (\ )\\
\semantic{$a_0$ \ ":" \ $t_0$ \ "," \ $\mathit{ltf}$}_\Gamma = s :\Leftrightarrow
    & T_0 = \semantic{$t_0$}_\Gamma\\
    &\land s = ((a_0,T_0), \dots, (a_n,T_n))\\
    &\land \semantic{$\mathit{ltf}$}_\Gamma = ((a_1,T_1), \dots, (a_n,T_n))\\
    &\text{where } n\in\mathbb{N} \text{ and } T_i\in\mathcal{T},a_i\in\mathcal{V} \text{ for all } i \in \mathbb{N}_0^n
\end{aligned}
$$
  
Let $s\in\mathcal{T}^*$ for the following function.

$$
\begin{aligned}
\semantic{.}_\Gamma:&\mf{<list-type>}\to\mathcal{T}^*\\
\semantic{""}_\Gamma = s :\Leftrightarrow
    & s = (\ )\\
\semantic{$t_0 \ \mathit{lt}$}_\Gamma = s :\Leftrightarrow
    &T_0 = \semantic{$t_0$}_\Gamma\\
    &\land \semantic{$lt$}_\Gamma =  (T_1,\dots,T_n)\\
    &\land s= (T_0,\dots,T_n)\\
    &\text{where } n\in\mathbb{N} \text{ and } T_i\in\mathcal{T} \text{ for all } i \in \mathbb{N}_0^n
\end{aligned}
$$

Let $s\in\mathcal{T}$ for the following function.

$$
\begin{aligned}
\semantic{.}_\Gamma:&\mf{<type>}\to\mathcal{T}\\
\semantic{"Bool"}_\Gamma = s :\Leftrightarrow
    & s = \mathit{Bool}\\
\semantic{"Int"}_\Gamma = s :\Leftrightarrow
    & s = \mathit{Int}\\
\semantic{"List" \ $t$}_\Gamma = s :\Leftrightarrow
    & T=\semantic{t}_\Gamma \land s = \mathit{List} \ T\\
    &\text{where } T\in\mathcal{T}\\
\semantic{"(" \ $t_1$ "," \ $t_2$ \ ")"}_\Gamma = s :\Leftrightarrow
    & T_1 = \semantic{$t_1$}_\Gamma \land T_2 = \semantic{$t_2$}_\Gamma \land s = (T_1,T_2)\\
    &\text{where } T_1,T_2\in\mathcal{T}\\
\semantic{"\{" \ $\mathit{ltf}$ \ "\}"}_\Gamma = s :\Leftrightarrow
    & \semantic{$\mathit{ltf}$}_\Gamma = ((a_1,T_1),\dots,(a_n,T_n))\\
    &\land s= \{a_1:T_1,\dots,a_n:T_n\}\\
    &\text{where } n\in\mathbb{N} \text{ and } T_i\in\mathcal{T},a_i\in\mathcal{V} \text{ for all } i \in \mathbb{N}_0^n\\
\semantic{$t_1$ \ "->" \ $t_2$}_\Gamma = s :\Leftrightarrow
    & \semantic{$t_1$}_\Gamma = T_1 \land \semantic{$t_2$}_\Gamma = T_2 \land s= T_1 \to T_2\\
\semantic{$c \ \mathit{lt}$}_\Gamma = s :\Leftrightarrow
    & (c,T)\in\Gamma\\
    &\land (T_1,\dots,T_n) = \semantic{$\mathit{lt}$}_\Gamma\\
    &\land T' = \overline{T} \ T_1 \dots T_n\\
    &\land s = T'\\
    &\text{where } n\in\mathbb{N} , T,T'\in\mathcal{T} \text{ and } T_i\in\mathcal{T} \text{ for all } i \in \mathbb{N}_1^n\\
\semantic{$a$}_\Gamma = s :\Leftrightarrow
    & s = \forall b.b
\end{aligned}
$$
```

We have already seen the pattern matching predicate in the last section. It is now time to actually define its meaning.

```{definition, name="Pattern Semantic"}
\begin{letIn}
$\Gamma$ be a type context and let $\Theta,\Theta_1,\Theta_2,\Theta_3$ be variable contexts. Let $p,p_1,p_2\in\mf{<pattern>}$, $\mathit{lpl}\in\mf{<list-pattern-list>}$, $\mathit{lps}\in\mf{<list-pattern-sort>}$ and $\mathit{lpv}\in\mf{<list-pattern-vars>}$. Let $b\in\mf{<bool>}$ and $i\in\mf{<int>}$. Let $c,a\in\mathcal{V}$.
\end{letIn}

Let $s\in\bigcup_{T\in\mathcal{T}} \text{value}_\Gamma(\mathit{List} \ T))$ for the following predicate.

$$
\begin{aligned}
\text{match}_\Theta:&(\bigcup_{T\in\mathcal{T}} \text{value}_\Gamma(\mathit{List} \ T))\times\mf{<list-pattern-list>}\\
\text{match}_\Theta(s,\mf{""}):\Leftrightarrow& [ \ ] = s\\
\text{match}_{\Theta_3}(s,p \ \mf{","} \ \mathit{lpl}):\Leftrightarrow& [a_0,\dots,a_n] = s\\
    &\land \text{match}_{\Theta_1}(a_0,p) \land \text{match}_{\Theta_2}(a_1,\dots,a_n,\mathit{lpl})\\
    &\land \varnothing = \Theta_1 \cap \Theta_2 \land \Theta_3 = \Theta_1 \cup \Theta_2\\
    &\text{where } n\in\mathbb{N} \text{ and } a_i\in\mathcal{V} \text{ for all } i \in \mathbb{N}_0^n.
\end{aligned}
$$

Let $s\in\bigcup_{T\in\mathcal{T}}\text{value}_\Gamma(T)^*$ for the following predicate.
      
$$
\begin{aligned}
\text{match}_\Theta:&\bigcup_{T\in\mathcal{T}}\text{value}_\Gamma(T)^*\times\mf{<list-pattern-sort>}\\
\text{match}_\Theta(s,\mf{""}) :\Leftrightarrow& ( \ ) = s\\
\text{match}_{\Theta_3}(s,p \ \mathit{lps}) :\Leftrightarrow& (s_1,\dots,s_n) = s\\
    &\land \text{match}_{\Theta_1}(s_1,p) \land \text{match}_{\Theta_2}(s_2,\dots,s_n,\mathit{lps})\\
    &\land \varnothing = \Theta_1 \cap \Theta_2 \land \Theta_3 = \Theta_1 \cup \Theta_2\\
    &\text{where } n\in\mathbb{N} \text{ and } s_i\in\text{value}(T) \text{ with } T\in\mathcal{T} \text{ for all } i \in \mathbb{N}_0^n.\\
\end{aligned}
$$

Let $s\in\mathcal{V}^*$ for the following function.

$$
\begin{aligned}
\semantic{.} :& \mf{<list-pattern-vars>} \to \mathcal{V}^*\\
\semantic{""} = s :\Leftrightarrow& s = (\ )\\
\semantic{$a_0 \ \mathit{lpv}$} = s:\Leftrightarrow& (a_1,\dots,a_n) = \semantic{$\mathit{lpv}$} \land (a_0,\dots,a_n) = s\\
    &\text{where } n\in\mathbb{N} \text{ and } a_i\in\mathcal{V} \text{ for all } i \in \mathbb{N}_0^n.
\end{aligned}
$$

Let $s\in\bigcup_{T\in\mathcal{T}}\text{value}_\Gamma(T)$ for the following predicate.
  
$$
\begin{aligned}
\text{match}_\Theta:&\bigcup_{T\in\mathcal{T}}\text{value}_\Gamma(T)\times\mf{<pattern>}\\
\text{match}_\Theta(s,b) :\Leftrightarrow& \land b\in\mf{<bool>} \land s = \semantic{$b$}_{\Gamma,\varnothing}\\
\text{match}_\Theta(s,i) :\Leftrightarrow& \land i\in\mf{<int>} \land s = \semantic{$b$}_{\Gamma,\varnothing}\\
\text{match}_\Theta(s,\mf{"["} \ \mathit{lpl} \ \mf{"]"}) :\Leftrightarrow& \text{match}_\Theta(s,\mathit{lpl})\\
\text{match}_{\Theta_3}(s,\mf{"("} \ p_1 \ \mf{","} \ p_2 \ \mf{")"}) :\Leftrightarrow& (s_1,s_2) = s\\
    &\land \text{match}_{\Theta_1}(s_1,p_1) \land \text{match}_{\Theta_2}(s_2,p_2)\\
    &\land \varnothing = \Theta_1 \cap \Theta_2 \land \Theta_3 = \Theta_1 \cup \Theta_2\\
    &\text{where } s_1\in\text{value}(T_1),s_2\in\text{value}(T_2) \text{ for}\\
    &T_1,T_2\in\mathcal{T}\\
\text{match}_\Theta(s,c \ \mathit{lps}) :\Leftrightarrow& c \ s_1 \ \dots \ s_n = s \land \text{match}_\Theta((s_1,\dots,s_n),\mathit{lps})\\
    &\text{where } n\in\mathbb{N} \text{ and } s_i\in\text{value}(T) \text{ with } T\in\mathcal{T} \text{ for}\\
    &\text{all } i \in \mathbb{N}_0^n.\\
\text{match}_\Theta(s,a) :\Leftrightarrow& s\in\mathcal{V} \land \Theta = \{(a,s)\}\\
\text{match}_{\Theta_2}(s,p \ \mf{"as"} \ a) :\Leftrightarrow& \text{match}_{\Theta_1}(s,p)\\
    &\land \varnothing = \Theta_1\cap\{(a,s)\} \land \Theta_2 = \Theta_1\cup\{(a,s)\}\\
\text{match}_\Theta(s,\mf{"\{"} \ \mathit{lpv} \ \mf{"\}"}) :\Leftrightarrow& (a_1,\dots,a_n) = \semantic{$\mathit{lpv}$}\\
    &\land \{a_1=e_1,\dots,a_n=e_n\}= s\\
    &\land \Theta = \{(a_1,e_1),\dots,(a_n,e_n)\}\\
    &\text{where } n\in\mathbb{N} \text{ and } a_i\in\mathcal{V} \text{ for all } i \in \mathbb{N}_0^n.\\
\text{match}_{\Theta_3}(s,p_1 \ \mf{"::"} \ p_2):\Leftrightarrow& (s_1,\dots,s_n)= s \land \text{match}_{\Theta_1}(s_1,p_1)\\
    &\land \text{match}_{\Theta_2}((s_2,\dots,s_n),p_2)\\
    &\land \varnothing = \Theta_1 \cap \Theta_2 \land \Theta_3 = \Theta_1 \cup \Theta_2\\
    &\text{where } n\in\mathbb{N} \text{ and } s_i\in\text{value}(T) \text{ with } T\in\mathcal{T} \text{ for}\\
    &\text{all } i \in \mathbb{N}_0^n.\\
\text{match}_\Theta(\mf{"\_"}):\Leftrightarrow& \varnothing = \Theta
\end{aligned}
$$
```

An Elm program is nothing more than an expression. Semantics of an expression is therefore the heart piece of this section.

```{definition, name="Expression Semantic"}
\begin{letIn}
$\Gamma$ be a type context and let $\Delta,\Theta$ be variable contexts. Let $a,a_0,a_1\in\mathcal{V}$, $e,e_1,e_2,e_3\in\mf{<exp>}$. Let $\mathit{lef}\in\mf{<list-exp-field>}$, $t\in\mf{<type>}$, $p\in\mf{<pattern>}$, $\mathit{lc}\in\mf{<list-case>}$, $b\in\mf{<bool>}$, $\mathit{nr}\in\mathbb{N}$, $\mathit{le}\in\mf{<list-exp>}$ and $\mathit{mes}\in\mf{<maybe-expression-sign>}$.
\end{letIn}

Let $s\in(\mathcal{V}\times\bigcup_{T\in\mathcal{T}}\text{value}_\Gamma(T))^*$ for the following function.

$$
\begin{aligned}
\semantic{.}_{\Gamma,\Delta}:& \mf{<list-exp-field>} \to (\mathcal{V}\times\bigcup_{T\in\mathcal{T}}\text{value}_\Gamma(T))^*\\
\semantic{$a$ \ "=" \ $e$}_{\Gamma,\Delta} = s_1 :\Leftrightarrow
    &s_2 = \semantic{$e$}_{\Gamma,\Delta} \land ((a,s_2))= s_1\\
    &\text{where } s_2\in\text{value}_\Gamma(T) \text{ for } T\in\mathcal{T}\\
\semantic{$a_1$ \ "=" \ $e$ \ "," \ $lef$}_{\Gamma,\Delta} = s_3 :\Leftrightarrow
    & ((a_1,s_1)) = \semantic{$a$ \ "=" \ $e$}_{\Gamma,\Delta}\\
    &\land ((a_2,s_2),\dots,(a_n,s_n)) = \semantic{$lef$}_{\Gamma,\Delta}\\
    &\land ((a_1,s_1),\dots,(a_n,s_n)) = s_3\\
    &\text{where } \ n\in\mathbb{N} \text{ and } a_i\in\mathcal{V},s_i\in\text{value}_\Gamma(T_i)\\
    &\text{ for } T_i\in\mathcal{T} \text{ for } i\in\mathbb{N}_0^n
\end{aligned}
$$

$$
\begin{aligned}
\semantic{.}_{\Gamma,\Delta}:& \mf{<maybe-exp-sign>}\to(\ )\\
\semantic{""}_{\Gamma,\Delta} = s :\Leftrightarrow
    & (\ )= s\\
\semantic{$a$ \ ":" $t$ \ ";"}_{\Gamma,\Delta} = s :\Leftrightarrow
    & (\ ) = s
\end{aligned}
$$

Let $s\in\bigcup_{T\in\mathcal{T}}\text{value}_\Gamma(T))$ for the following function.

$$
\begin{aligned}
\semantic{.}_{\Gamma,\Delta}:& \mf{<exp>}\to\mf{<list-case>}\to \bigcup_{T\in\mathcal{T}}\text{value}_\Gamma(T))\\
\semantic{$e_1,p$ \ "->" \ $e_2$}_{\Gamma,\Delta} = s :\Leftrightarrow
    & \text{match}_{\Theta}(e_1,p) \land \semantic{$e_2$}_{\Gamma,\Delta\cup\Theta} = s\\
\semantic{$e_1,p$ \ "->" \ $e_2$ \ ";" \ $lc$}_{\Gamma,\Delta} = s :\Leftrightarrow
    & s = 
      \begin{cases}
        \semantic{$e_2$}_{\Gamma,\Delta\cup\Theta} &\text{if }\text{match}_{\Theta}(e_1,p)\\
        \semantic{$e_1,lc$}_{\Gamma,\Delta} &\text{else }
      \end{cases}
\end{aligned}
$$
      
Let $s\in\text{value}_\varnothing(\mathit{Bool})$ for the following function.
      
$$
\begin{aligned}
\semantic{.}:&\mf{<Bool>}\to\text{value}_\varnothing(\mathit{Bool})\\
\semantic{$b$} = s :\Leftrightarrow
    & \begin{cases}
        \mathit{True}&\text{if }b = \mf{"True"}\\
        \mathit{False}&\text{if }b = \mf{"False"}
      \end{cases}
\end{aligned}
$$
          
Let $s\in\text{value}_\varnothing(\mathit{Int})$ for the following function.
  
$$
\begin{aligned}
\semantic{.}:&\mf{<int>}\to\text{value}_\varnothing(\mathit{Int})\\
\semantic{"0"} = s :\Leftrightarrow
    & 0 = s\\
\semantic{"-" \ $\mathit{nr}$} = s :\Leftrightarrow
    & \mathit{Neg} \ \mathit{Succ}^\mathit{nr} \ 1\\
\semantic{$\mathit{nr}$} = s :\Leftrightarrow
    & \mathit{Pos} \ \mathit{Succ}^\mathit{nr} \ 1
\end{aligned}
$$
  
Let $s\in\bigcup_{T\in\mathcal{T}}\text{value}_\Gamma(T))^*$ for the following function.

$$
\begin{aligned}
\semantic{.}_{\Gamma,\Delta}:&\mf{<list-exp>}\to\bigcup_{T\in\mathcal{T}}\text{value}_\Gamma(T))^*\\
\semantic{""}_{\Gamma,\Delta} = s :\Leftrightarrow
    & (\ ) = s\\
\semantic{$e$ \ "," \ $\mathit{le}$}_{\Gamma,\Delta} = s :\Leftrightarrow
    & s_1 = \semantic{$e$}_{\Gamma,\Delta} \land (s_2,\dots,s_n) = \semantic{$\mathit{le}$}_{\Gamma,\Delta} \land (s_1,\dots,s_n) = s\\
    & \text{where } \ n\in\mathbb{N} \ \text{ and }\ s_i\in\text{value}_\Gamma(T_i),T_i\in\mathcal{T} \text{ for each } i\in\mathbb{N}_0^n
\end{aligned}
$$
      
Let $s\in\bigcup_{T\in\mathcal{T}}\text{value}_\Gamma(T)$ for the following function.
      
$$\semantic{.}_{\Gamma,\Delta}:\mf{<exp>}\to\bigcup_{T\in\mathcal{T}}\text{value}_\Gamma(T)$$
$$\begin{aligned}
\semantic{"foldl"}_{\Gamma,\Delta} = s:\Leftrightarrow
    & s = \lambda f. \lambda e_1. \lambda l_1.\\
    &\small\begin{cases}
        e_1 &\text{if } [\ ] = l_1\\
        f(e_2, s(f,e_1,l_2)) & \text{if } \textit{Cons} \ e_2 \ l_2 = l_1
      \end{cases}\\
    &\text{where } \ e_1\in\text{value}_\Gamma(T_1),e_2\in\text{value}_\Gamma(T_2)\\
    &\text{ and } l_1,l_2\in\text{value}_\Gamma(\mathit{List} \ T_2) \text{ and }\\
    &f\in\text{value}_\Gamma(T_2\to T_1 \to T_1) \text{ for } T_1,T_2\in\mathcal{T}
\end{aligned}
$$
$$
\begin{aligned}
\semantic{"(::)"}_{\Gamma,\Delta} = s:\Leftrightarrow
    & s = \lambda e. \lambda l. \textit{Cons} \ e \ l\\
    & \text{where } \ e\in\text{value}_\Gamma(T) \text{ and } \ l\in\text{value}_\Gamma(\mathit{List} \ T)\\
    & \text{ for } T\in\mathcal{T}
\end{aligned}
$$
$$
\begin{aligned}
\semantic{"(+)"}_{\Gamma,\Delta} = s:\Leftrightarrow
    & s = \lambda n.\lambda m. n + m\\
    & \text{where } n,m\in\mathbb{N}
\end{aligned}
$$
$$
\begin{aligned}
\semantic{"(-)"}_{\Gamma,\Delta} = s:\Leftrightarrow
    & s = \lambda n.\lambda m. n - m\\
    & \text{where } n,m\in\mathbb{N}
\end{aligned}
$$
$$
\begin{aligned}
\semantic{"(*)"}_{\Gamma,\Delta} = s:\Leftrightarrow
    & s = \lambda n.\lambda m. n * m\\
    & \text{where } n,m\in\mathbb{N}
\end{aligned}
$$
$$
\begin{aligned}
\semantic{"(//)"}_{\Gamma,\Delta} = s:\Leftrightarrow
    & \begin{cases}s = \lambda n.\lambda m. \Big\lfloor \frac{n}{m} \Big\rfloor& \text{if } m \neq 0\\
        0& \text{else}\end{cases}\\
    & \text{where } n,m\in\mathbb{N}
\end{aligned}
$$
$$
\begin{aligned}
\semantic{"(<)"}_{\Gamma,\Delta} = s:\Leftrightarrow
    & s = \lambda n.\lambda m. n < m\\
    & \text{where } n,m\in\mathbb{N}
\end{aligned}
$$
$$
\begin{aligned}
\semantic{"(==)"}_{\Gamma,\Delta} = s:\Leftrightarrow
    & s = \lambda n.\lambda m. (n = m)\\
    & \text{where } n,m\in\mathbb{N}
\end{aligned}
$$
$$
\begin{aligned}
\semantic{"not"}_{\Gamma,\Delta} = s:\Leftrightarrow
    & s = \lambda b. \neg b\\
    & \text{where }b\in\text{value}_\Gamma(\mathit{Bool})
\end{aligned}
$$
$$
\begin{aligned}
\semantic{"(\&\&)"}_{\Gamma,\Delta} = s:\Leftrightarrow
    & s = \lambda b_1.\lambda b_2. b_1 \land b_2\\
    & \text{where }b_1,n_2\in\text{value}_\Gamma(\mathit{Bool})
\end{aligned}
$$
$$
\begin{aligned}
\semantic{"(||)"}_{\Gamma,\Delta} = s:\Leftrightarrow
    & s = \lambda b_1.\lambda b_2. b_1 \lor b_2\\
    & \text{where }b_1,n_2\in\text{value}_\Gamma(\mathit{Bool})
\end{aligned}
$$
$$
\begin{aligned}
\semantic{$e_1$ \ "|>" \ $e_2$}_{\Gamma,\Delta} = s:\Leftrightarrow
    & s' = \semantic{$e_1$}_{\Gamma,\Delta} \land f = \semantic{$e_2$}_{\Gamma,\Delta} \land f(s_1) = s\\
    & \text{where }f\in\text{value}(T_1\to T_2),s'\in\text{value}(T_1)\text{ for }T_1,T_2\in\mathcal{T}
\end{aligned}
$$
$$
\begin{aligned}
\semantic{$e_1$ \ ">>" \ $e_2$}_{\Gamma,\Delta} = s:\Leftrightarrow
    & g = \semantic{$e_1$}_{\Gamma,\Delta} \land f = \semantic{$e_2$}_{\Gamma,\Delta} \land
 f\circ g=s\\
    & \text{where } g\in\text{value}(T_1\to T_2),f\in\text{value}(T_2\to T_3)\text{ for }\\
    & T_1,T_2,T_2\in\mathcal{T}
\end{aligned}
$$
$$
\begin{aligned}
 \Bigg\llbracket\begin{aligned}
 &\mf{"if"} \ e_1 \ \mf{"then"}\\
 & \ e_2 \ \mf{"else"} \ e_3
 \end{aligned}\Bigg\rrbracket_{\Gamma,\Delta} = s:\Leftrightarrow
    & b = \semantic{$e_1$}_{\Gamma,\Delta} \land s = 
      \begin{cases}
        \semantic{$e_2$}_{\Gamma,\Delta} & \text{if } b\\
        \semantic{$e_3$}_{\Gamma,\Delta} & \text{if } \neg b
      \end{cases}\\
    & \text{where } b\in\text{value}(\mathit{Bool})
\end{aligned}
$$
$$
\begin{aligned}
\semantic{"\{" \ $\mathit{lef}$ \ "\}"}_{\Gamma,\Delta} = s:\Leftrightarrow
    & ((a_1,s_1),\dots,(a_n,s_n))=\semantic{$\mathit{lef}$}_{\Gamma,\Delta}\\
    &\land \{a_1=s_1,\dots,a_n=s_n\}= s\\
    &\text{where } n\in\mathbb{N} \text{ and } a_i\in\mathcal{V},s_i\in\text{value}(T_i),T_i\in\mathcal{T} \text{ for }i\in\mathbb{N}_0^n
 \end{aligned}
$$
$$
\begin{aligned}
\semantic{"\{ \}"}_{\Gamma,\Delta} = s:\Leftrightarrow
    & \{ \}= s
 \end{aligned}
$$
$$
\begin{aligned}
\semantic{"\{" \ $a$ \ "|" \ $\mathit{lef}$ \ "\}"}_{\Gamma,\Delta} = s:\Leftrightarrow
    & ((a_1,s_1),\dots,(a_n,s_n))=\semantic{$\mathit{lef}$}_{\Gamma,\Delta}\\
    &\land (a,\small\begin{Bmatrix*}[l]a_1=\_,\dots,a_n=\_,\\a_{n+1}=s_{n+1},\dots,a_m=s_m\end{Bmatrix*})\in\Delta\\
    &\land \{a_1=s_1,\dots,a_m=s_m\}= s\\
    &\text{where } n,m\in\mathbb{N} \text{ such that } n \leq m \text{ and } a_i\in\mathcal{V},\\
    &s_i\in\text{value}(T_i),T_i\in\mathcal{T} \text{ for }i\in\mathbb{N}_0^m
\end{aligned}
$$
$$
\begin{aligned}
\semantic{$a_0$ \ "." \ $a_1$}_{\Gamma,\Delta} = s :\Leftrightarrow
    & (a_0,\{a_1:s_1,\dots\})\Delta \land s' = s\\
    & \text{where } s'\in\text{value}(T) \text{for } T\in\mathcal{T}
\end{aligned}
$$
$$
\begin{aligned}
\Bigg\llbracket\begin{aligned}
 &\mf{"let"} \ \mathit{mes} \ a \ \mf{"="} \ e_1 \\
 &\mf{"in"} \ e_2
 \end{aligned}\Bigg\rrbracket_{\Gamma,\Delta} = s :\Leftrightarrow
    & s' = \semantic{$e_1$}_{\Gamma,\Delta} \ \land \semantic{$e_2$}_{\Gamma,\Delta\cup\{(a,s')\}} = s\\
    & \text{where } s' \in\text{value}(T) for T\in\mathcal{T}
\end{aligned}
$$
$$
\begin{aligned}
\Bigg\llbracket\begin{aligned}
 &\mf{"case"} \ e \ \mf{"of"} \\
 &\mf{"["} \ \mathit{lc} \ \mf{"]"}
 \end{aligned}\Bigg\rrbracket_{\Gamma,\Delta} = s :\Leftrightarrow
    & \semantic{$e$,$\mathit{lc}$}_{\Gamma,\Delta}= s
 \end{aligned}
$$
$$
\begin{aligned}
\semantic{$e_1 \ e_2$}_{\Gamma,\Delta} = s:\Leftrightarrow
    & s_1 = \semantic{$e_1$}_{\Gamma,\Delta} \land s_2 = \semantic{$e_2$}_{\Gamma,\Delta}\land s_1(s_2) = s\\
    & \text{where } s_1 \in\text{value}_\Gamma(T_1\to T_2) \text{ and } s_2\in\text{value}_\Gamma(T_1) \text{for }T_1,T_2\in\mathcal{T} 
 \end{aligned}
$$
$$
\begin{aligned}
 \semantic{$b$}_{\Gamma,\Delta} = s:\Leftrightarrow
    & \semantic{$b$} = s
 \end{aligned}
$$
$$
\begin{aligned}
\semantic{$i$}_{\Gamma,\Delta} = s:\Leftrightarrow
    & \semantic{$i$} = s
 \end{aligned}
$$
$$
\begin{aligned}
\semantic{"[" \ $\mathit{le}$ \ "]"}_{\Gamma,\Delta} = s:\Leftrightarrow
    & (s_1,\dots,s_n) = \semantic{$\mathit{le}$}_{\Gamma,\Delta} \land [s_1,\dots,s_n]= s\\
    & \text{where }n\in\mathbb{N} \text{ and } s_i\in\text{value}_\Gamma(T) \text{ for } T\in\mathcal{T}
\end{aligned}
$$
$$
\begin{aligned}
\semantic{"(" \ $e_1$ \ "," \ $e_2$ \ ")"}_{\Gamma,\Delta} = s:\Leftrightarrow
    & s_1=\semantic{$e_1$} \land s_2=\semantic{$e_2$} \land (s_1,s_2) = s\\
    & \text{where }s_1\in\text{value}_\Gamma(T_1) \text{ and } s_2\in\text{value}_\Gamma(T_1)
\end{aligned}
$$
$$
\begin{aligned} 
\semantic{"\textbackslash" \ $p$ \ "->" \ $e$}_{\Gamma,\Delta} = s:\Leftrightarrow
    & \text{match}_\Theta(s_1,p)\land s_2=\semantic{$e$}\land \lambda s_1.s_2 = s\\
    & \text{where }s_1\in\text{value}_\Gamma(T_1) \text{ and } s_2\in\text{value}_\Gamma(T_1)
\end{aligned}
$$
$$
\begin{aligned} 
\semantic{$c$}_{\Gamma,\Delta} = s:\Leftrightarrow
    & (c,s)\in\Delta\\
\end{aligned}
$$
$$
\begin{aligned} 
\semantic{$a$}_{\Gamma,\Delta} = s:\Leftrightarrow
    & (a,s)\in\Delta
\end{aligned}
$$
```

Statements are, semantically speaking, just functions that either map the type- or variable-context. 

```{definition, name="Statement Semantic"}
\begin{letIn}
$\Gamma$ be a type context. Let $a,a_0\in\mathcal{V}$, $t\in\mf{<type>}$, $\mathit{lsv}\in\mf{<list-statement-var>}$, $\mathit{lt}\in\mf{<list-type>}$, $\mathit{lss}\in\mf{<list-statement-sort>}$, $\mathit{st}\in\mf{<statement>}$, $\mathit{ls}\in\mf{<list-statement>}$, $\mathit{mss}\in\mf{<maybe-statement-sign>}$ and $\mathit{mms}\in\mf{<maybe-main-sign>}$. Let $\mathcal{S}$ be the class of all finite sets.
\end{letIn}

Let $s\in\mathcal{V}^*$ for the following function.

$$
\begin{aligned}
\semantic{.}:&\mf{<list-statement-var>}\to\mathcal{V}^*\\
\semantic{""} = s:\Leftrightarrow
    & (\ ) = s\\
\semantic{$a_0$ \ $\mathit{lsv}$} = s:\Leftrightarrow
    & (a_1,\dots,a_n) = \semantic{$\mathit{lsv}$} \land (a_0,\dots,a_n)= s\\
    & \text{where } \ n\in\mathbb{N} \text{ and } a_i\in\mathcal{V}\text{ for }i\in\mathbb{N}_0^n
\end{aligned}
$$

Let $s\in(\mathcal{V}\times\mathcal{T}^*)^*$ for the following function.
  
$$
\begin{aligned}
\semantic{.}_\Gamma:&\mf{<list-statement-sort>}\to(\mathcal{V}\times\mathcal{T}^*)^*\\
\semantic{$a$ \ $\mathit{lt}$}_\Gamma = s:\Leftrightarrow
    & l = \semantic{$\mathit{lt}$}_\Gamma \land ((a,l))=s\\
    & \text{where } l\in\mathcal{T}^*\\
\semantic{$a_0$ \ $\mathit{lt}$ \ $\mathit{lss}$}_\Gamma = s :\Leftrightarrow
    & ((a_1,l_1),\dots,(a_n,l_n))= \semantic{$\mathit{lss}$}\\
    &\land \ l_0 = \semantic{$\mathit{lt}$}_\Gamma\\
    &\land ((a_0,l_0),\dots,(a_n,l_n)) = s\\
    &\text{where } n\in\mathbb{N} \text{ and } a_i\in\mathcal{V},l_i\in\mathcal{T}^* \text{ for } i\in\mathbb{N}
\end{aligned}
$$
  
Let $s\in((\mathcal{V}\nrightarrow\mathcal{T})\times(\mathcal{V}\nrightarrow\mathcal{S}))\to((\mathcal{V}\nrightarrow\mathcal{T})\times(\mathcal{V}\nrightarrow\mathcal{S}))$ for the following function.  

$$
\begin{aligned}
\semantic{.}:\mf{<list-state}&\mf{ment>}\to((\mathcal{V}\nrightarrow\mathcal{T})\times(\mathcal{V}\nrightarrow\mathcal{S}))\to((\mathcal{V}\nrightarrow\mathcal{T})\times(\mathcal{V}\nrightarrow\mathcal{S}))\\
\semantic{""} = s:\Leftrightarrow
    & \mathit{id} = s\\
\semantic{$st$ \ "," \ $\mathit{ls}$} = s:\Leftrightarrow
    & f = \semantic{$st$} \land g = \semantic{$\mathit{ls}$} \land g\circ f= s\\
    & \text{where } f,g\in\small{((\mathcal{V}\nrightarrow\mathcal{T})\times(\mathcal{V}\nrightarrow\mathcal{S}))\to((\mathcal{V}\nrightarrow\mathcal{T})\times(\mathcal{V}\nrightarrow\mathcal{S}))}
\end{aligned}
$$

$$
\begin{aligned}
\semantic{.}:&\mf{<maybe-statement-sign>}\to(\ )\\
\semantic{""} = s:\Leftrightarrow
    & (\ )= s\\
\semantic{$a$ \ ":" \ $t$ ";"} = s:\Leftrightarrow
    & (\ )= s
\end{aligned}
$$
  
Let $s\in((\mathcal{V}\nrightarrow\mathcal{T})\times(\mathcal{V}\nrightarrow\mathcal{S}))\to((\mathcal{V}\nrightarrow\mathcal{T})\times(\mathcal{V}\nrightarrow\mathcal{S}))$ for the following function.  
  
$$
\begin{aligned}
\semantic{.}:\mf{<statement>} \to&((\mathcal{V}\nrightarrow\mathcal{T})\times(\mathcal{V}\nrightarrow\mathcal{S}))\to((\mathcal{V}\nrightarrow\mathcal{T})\times(\mathcal{V}\nrightarrow\mathcal{S}))\\
\semantic{$mss$ \ $a$ \ "=" \ $e$}(\Gamma,\Delta) = s :\Leftrightarrow
    & s' = \semantic{$e$}_{\Gamma,\Delta} \land (\Gamma,\Delta\cup\{(a,s')\})= s\\
    & \text{where } s'\in \text{value}(T) \text{ for } T\in\mathcal{T}\\
\Bigg\llbracket\begin{aligned}
&\mf{"type } \mf{alias"} \\
& c \ \mathit{lsv} \ \mf{"="} \ t
\end{aligned}\Bigg\rrbracket(\Gamma,\Delta) = s :\Leftrightarrow& T = \semantic{t}_\Gamma \land (\Gamma\cup\{(c,T)\},\Delta)= s\\
\Bigg\llbracket\begin{aligned}
&\mf{"type"} \ c \\
&\mathit{lsv} \ \mf{"="} \ \mathit{lss}
  \end{aligned}\Bigg\rrbracket(\Gamma_1,\Delta_2) = s:\Leftrightarrow& ((c_1,(T_{1,1},\dots,T_{1,k_1})),\dots,(c_n,(T_{n,1},\dots,T_{n,k_n})))\\
&\land T_1 = \mu C.c_1 T_{1,1} \dots T_{1,k_1} | \dots | c_n T_{n,1} \dots T_{n,k_n}\\
&\land (a_1,\dots,a_m) = \semantic{$\mathit{lsv}$}\\
&\land T_2 = \forall a_1. \dots \forall a_m T_1\\
&\land \Gamma_2 = \Gamma_1\cup\{(c,T_2)\}\\
&\land \Delta_2 = \begin{Bmatrix*}[l]
\small{(c_1,\lambda t_{1,1}. \dots,\lambda t_{1,k_1}.c_1 t_{1,1} \dots t_{1,k_1})}\\
\vdots\\
\small{(c_n,\lambda t_{n,1}. \dots,\lambda t_{n,k_n}.c_1 t_{n,1} \dots t_{n,k_n})}
\end{Bmatrix*}\\
&\land \Delta_3 = \Delta_1\cup\Delta_2\\
&\land (\Gamma_2,\Delta_3) = s\\
&\text{where }n,m\in\mathbb{N} \text{ and } k_i\in\mathbb{N},c_i,a_j\in\mathcal{V},T_{i,l_i}\in\mathcal{T}\\
&\text{ for }i\in\mathbb{N}_1^n,j\in\mathbb{N}_1^m,l_i\in\mathbb{N}_0^{k_i}
\end{aligned}
$$
  
$$
\begin{aligned}
\semantic{.}:&\mf{<maybe-main-sign>}\to(\ )\\
\semantic{""} = s:\Leftrightarrow& (\ )= s\\
\semantic{"main : " \ $t$ \ ";"} = s:\Leftrightarrow& (\ ) = s
\end{aligned}
$$

Let $s\in\bigcup_{T\in\mathcal{T}}\text{value}_\Gamma(T)$ for the following function.  
$$
\begin{aligned}
\semantic{.}:&\mf{<program>}\to\bigcup_{T\in\mathcal{T}}\text{value}_\Gamma(T)\\
\semantic{$\mathit{ls}$ \ $\mathit{mms}$ \ "main = " \ $e$} = s:\Leftrightarrow& (\Gamma,\Delta) = \semantic{$\mathit{ls}$}(\varnothing,\varnothing) \land \semantic{$e$}_{\Gamma,\Delta} = s\\
    & \text{where }  \Gamma \text{ is a type context and } \Delta \text{ is a variable}\\
    & \text{context.}
\end{aligned}
$$
```